riscV/Asm.v
@@ -1085,54 +1085,22 @@ Definition loc_external_result (sg: signature) : rpair preg :=
 
 (** Execution of the instruction at [rs PC]. *)
 
-Inductive stackframe: Type :=
-  | Stackframe:
-      forall (f: block)       (**r pointer to calling function *)
-        (retaddr: ptrofs) (**r Asm return address in calling function *)
-        (sp: val),         (**r stack pointer in calling function *)
-      stackframe.
-
-Definition stack := list stackframe.
-
 Inductive state: Type :=
-  | State: stack -> regset -> mem -> state.
-
-Definition exec_instr_stack f i rs m st : outcome * stack :=
-  let oc := exec_instr f i rs m in
-  match oc with
-  | Stuck => (Stuck, st)
-  | Next rs' m' => (Next rs' m',
-                   let pc' := rs' # PC in
-                   let sp' := rs' # SP in
-                   match i with
-                   | Pjal_s _ _ | Pjal_r _ _ =>
-                              match rs # RA with
-                              | Vptr f retaddr => Stackframe f retaddr sp' :: st
-                              | _ => st
-                              end
-                   | _ =>
-                     match st with
-                     | nil => st
-                     | Stackframe f retaddr sp :: st' =>
-                       if Val.eq (Vptr f retaddr) pc' && Val.eq sp sp' then st'
-                       else st
-                     end
-                   end)
-  end.
+  | State: regset -> mem -> state.
 
 Inductive step: state -> trace -> state -> Prop :=
   | exec_step_internal:
-      forall b ofs f i rs m rs' m' b' ofs' fd st st',
+      forall b ofs f i rs m rs' m' b' ofs' fd,
       rs PC = Vptr b ofs ->
       Genv.find_funct_ptr ge b = Some (Internal f) ->
       find_instr (Ptrofs.unsigned ofs) (fn_code f) = Some i ->
-      exec_instr_stack f i rs m st = (Next rs' m', st') ->
+      exec_instr f i rs m = Next rs' m' ->
       forall (NEXTPC: rs' PC = Vptr b' ofs'),
       forall (NEXTFUN: Genv.find_funct_ptr ge b' = Some fd),
-      forall (ALLOWED: Policy.allowed_call pol f.(fn_comp) fd),
-      step (State st rs m) E0 (State st' rs' m')
+    forall (ALLOWED: Policy.allowed_call pol f.(fn_comp) fd),
+      step (State rs m) E0 (State rs' m')
   | exec_step_builtin:
-      forall b ofs f ef args res rs m vargs t vres rs' m' st,
+      forall b ofs f ef args res rs m vargs t vres rs' m',
       rs PC = Vptr b ofs ->
       Genv.find_funct_ptr ge b = Some (Internal f) ->
       find_instr (Ptrofs.unsigned ofs) f.(fn_code) = Some (Pbuiltin ef args res) ->
@@ -1143,9 +1111,9 @@ Inductive step: state -> trace -> state -> Prop :=
               (set_res res vres
                 (undef_regs (map preg_of (destroyed_by_builtin ef))
                    (rs#X31 <- Vundef))) ->
-      step (State st rs m) t (State st rs' m')
+      step (State rs m) t (State rs' m')
   | exec_step_external:
-      forall b ef args res rs m t rs' m' cp st,
+      forall b ef args res rs m t rs' m' cp,
       rs PC = Vptr b Ptrofs.zero ->
       Genv.find_funct_ptr ge b = Some (External ef) ->
       forall COMP: Genv.find_comp ge (rs RA) = Some cp,
@@ -1153,7 +1121,7 @@ Inductive step: state -> trace -> state -> Prop :=
       external_call ef ge cp args m t res m' ->
       extcall_arguments rs m (ef_sig ef) args ->
       rs' = (set_pair (loc_external_result (ef_sig ef) ) res (undef_caller_save_regs rs))#PC <- (rs RA) ->
-      step (State st rs m) t (State st rs' m').
+      step (State rs m) t (State rs' m').
 
 End RELSEM.
 
@@ -1168,13 +1136,13 @@ Inductive initial_state (p: program): state -> Prop :=
         # SP <- Vnullptr
         # RA <- Vnullptr in
       Genv.init_mem p = Some m0 ->
-      initial_state p (State nil rs0 m0).
+      initial_state p (State rs0 m0).
 
 Inductive final_state: state -> int -> Prop :=
-  | final_state_intro: forall rs m r st,
+  | final_state_intro: forall rs m r,
       rs PC = Vnullptr ->
       rs X10 = Vint r ->
-      final_state (State st rs m) r.
+      final_state (State rs m) r.
 
 Definition semantics (pol: policy) (p: program) :=
   Semantics (step pol) (initial_state p) final_state (Genv.globalenv p).
@@ -1218,10 +1186,10 @@ Ltac Equalities :=
   discriminate.
   discriminate.
   assert (vargs0 = vargs) by (eapply eval_builtin_args_determ; eauto). subst vargs0.
-  exploit external_call_determ. eexact H5. eexact H14. intros [A B].
+  exploit external_call_determ. eexact H5. eexact H11. intros [A B].
   split. auto. intros. destruct B; auto. subst. auto.
   assert (args0 = args) by (eapply extcall_arguments_determ; eauto). subst args0.
-  exploit external_call_determ. eexact H3. eexact H9. intros [A B].
+  exploit external_call_determ. eexact H3. eexact H8. intros [A B].
   split. auto. intros. destruct B; auto. subst. auto.
 - (* trace length *)
   red; intros. inv H; simpl.
